specs/Spec.Hash.Definitions.fst
@@ -59,6 +59,11 @@ let to_blake_alg (a:blake_alg) = match a with
   | Blake2S -> Spec.Blake2.Blake2S
   | Blake2B -> Spec.Blake2.Blake2B
 
+let to_hash_alg (a : Spec.Blake2.alg) =
+  match a with
+  | Spec.Blake2.Blake2S -> Blake2S
+  | Spec.Blake2.Blake2B -> Blake2B
+
 (** Maximum input data length. *)
 
 (* In bytes. *)
