specs/lemmas/Spec.Blake2.Lemmas.fsti
@@ -6,6 +6,13 @@ open Spec.Hash.Definitions
 open Spec.Agile.Hash
 open FStar.Mul
 
+val blake2_init_no_key_is_agile (a : hash_alg{is_blake a}) :
+  Lemma(
+    ((Spec.Blake2.blake2_init (to_blake_alg a) 0 Seq.empty (Spec.Blake2.max_output (to_blake_alg a))
+      <: words_state' a),
+     Spec.Agile.Hash.nat_to_extra_state a 0) ==
+      Spec.Agile.Hash.init a)
+
 val lemma_blake2_hash_equivalence
   (a:hash_alg{is_blake a}) (d:bytes{Seq.length d <= max_input_length a})
   : Lemma
